

# Lista 3

1) a)

	0	1	2	3	4
$x_i$	0	1.5	3.0	4.5	6.0
$f(x_i)$	0.001	0.016	0.028	0.046	0.057

$$P_n(x) = \sum_{i=0}^n l_i \cdot f(x_i) = L_0 \cdot f(x_0) + l_1 \cdot f(x_1) + l_2 \cdot f(x_2) + l_3 \cdot f(x_3) + l_4 \cdot f(x_4)$$

$$L_0 = \frac{(x-x_1)(x-x_2)(x-x_3)(x-x_4)}{(x_0-x_1)(x_0-x_2)(x_0-x_3)(x_0-x_4)} = \frac{(x-1.5)(x-3)(x-4.5)(x-6)}{121.5}$$

$$L_1 = \frac{(x-x_0)(x-x_2)(x-x_3)(x-x_4)}{(x_1-x_0)(x_1-x_2)(x_1-x_3)(x_1-x_4)} = \frac{(x)(x-3)(x-4.5)(x-6)}{-30.375}$$

$$L_2 = \frac{(x-x_0)(x-x_1)(x-x_3)(x-x_4)}{(x_2-x_0)(x_2-x_1)(x_2-x_3)(x_2-x_4)} = \frac{(x)(x-1.5)(x-4.5)(x-6)}{20.25}$$

$$L_3 = \frac{(x-x_0)(x-x_1)(x-x_2)(x-x_4)}{(x_3-x_0)(x_3-x_1)(x_3-x_2)(x_3-x_4)} = \frac{(x)(x-1.5)(x-3)(x-6)}{-30.375}$$

$$L_4 = \frac{(x-x_0)(x-x_1)(x-x_2)(x-x_3)}{(x_4-x_0)(x_4-x_1)(x_4-x_2)(x_4-x_3)} = \frac{(x)(x-1.5)(x-3)(x-4.5)}{121.5}$$

$$P(x) = 0.001 \cdot \frac{(x-1.5)(x-3)(x-4.5)(x-6)}{121.5} + 0.016 \cdot \frac{(x)(x-3)(x-4.5)(x-6)}{-30.375}$$

$$+ 0.028 \cdot \frac{(x)(x-1.5)(x-4.5)(x-6)}{20.25}$$

$$+ 0.046 \cdot \frac{(x)(x-1.5)(x-3)(x-6)}{-30.375} + 0.057 \cdot \frac{(x)(x-1.5)(x-3)(x-4.5)}{121.5}$$



$$b) P(1.1) = 0.001 \cdot \frac{(1.1-1.5) \cdot (1.1-3) \cdot (1.1-4.5) \cdot (1.1-6)}{121.5} +$$

$$0.016 \cdot \frac{(1.1-0) \cdot (1.1-3) \cdot (1.1-4.5) \cdot (1.1-6)}{-30.375} +$$

$$0.028 \cdot \frac{(1.1-0) \cdot (1.1-1.5) \cdot (1.1-4.5) \cdot (1.1-6)}{20.25} +$$

$$0.046 \cdot \frac{(1.1-0) \cdot (1.1-1.5) \cdot (1.1-3) \cdot (1.1-6)}{-30.375} +$$

$$0.057 \cdot \frac{(1.1-0) \cdot (1.1-1.5) \cdot (1.1-3) \cdot (1.1-4.5)}{121.5} =$$

$$0.0001 + 0.018 + (-0.001) + 0.006 + (-0.001) = \boxed{0.0131}$$

$$P(2.2) = 0.001 \cdot \frac{(2.2-1.5) \cdot (2.2-3) \cdot (2.2-4.5) \cdot (2.2-6)}{121.5} +$$

$$0.016 \cdot \frac{(2.2-0) \cdot (2.2-3) \cdot (2.2-4.5) \cdot (2.2-6)}{-30.375} +$$

$$0.028 \cdot \frac{(2.2-0) \cdot (2.2-1.5) \cdot (2.2-4.5) \cdot (2.2-6)}{20.25} +$$

$$0.046 \cdot \frac{(2.2-0) \cdot (2.2-1.5) \cdot (2.2-3) \cdot (2.2-6)}{-30.375} +$$

$$0.057 \cdot \frac{(2.2-0) \cdot (2.2-1.5) \cdot (2.2-3) \cdot (2.2-4.5)}{121.5} =$$

$$-0.00004 + 0.008 + 0.019 + (-0.007) + 0.001 = \boxed{0.021}$$

$$P(3.4) = 0.001 \cdot \frac{(3.4-1.5) \cdot (3.4-3) \cdot (3.4-4.5) \cdot (3.4-6)}{121.5} +$$

$$0.016 \cdot \frac{(3.4-0) \cdot (3.4-3) \cdot (3.4-4.5) \cdot (3.4-6)}{-30.375} +$$



$$0.028 \cdot \frac{(3.4-0) \cdot (3.4-1.5) \cdot (3.4-4.5) \cdot (3.4-6)}{20.25} +$$

$$0.046 \cdot \frac{(3.4-0) \cdot (3.4-1.5) \cdot (3.4-3) \cdot (3.4-6)}{-30.375} +$$

$$0.057 \cdot \frac{(3.4-0) \cdot (3.4-1.5) \cdot (3.4-3) \cdot (3.4-6)}{121.5} =$$

$$0.000018 + (-0.002) + 0.026 + 0.01 + (-0.001) = \boxed{0.033}$$

$$P(4.9) = 0.001 \cdot \frac{(4.9-1.5) \cdot (4.9-3) \cdot (4.9-4.5) \cdot (4.9-6)}{121.5} +$$

$$0.016 \cdot \frac{(4.9-0) \cdot (4.9-3) \cdot (4.9-4.5) \cdot (4.9-6)}{-30.375} +$$

$$0.028 \cdot \frac{(4.9-0) \cdot (4.9-1.5) \cdot (4.9-4.5) \cdot (4.9-6)}{20.25} +$$

$$0.046 \cdot \frac{(4.9-0) \cdot (4.9-1.5) \cdot (4.9-3) \cdot (4.9-6)}{-30.375} +$$

$$0.057 \cdot \frac{(4.9-0) \cdot (4.9-1.5) \cdot (4.9-3) \cdot (4.9-4.5)}{121.5} =$$

$$-0.000023 + 0.002 + (-0.01) + 0.052 + 0.005 = \boxed{0.049}$$

2) a)

	0	1	2
$x_i$	2	3	4
$f(x_i)$	0.6931	1.0986	1.3853

$$P_M(x) = \sum_{i=0}^2 L_i \cdot f(x_i) = L_0 \cdot f(x_0) + L_1 \cdot f(x_1) + L_2 \cdot f(x_2)$$

$$L_0 = \frac{(x-x_1)(x-x_2)}{(x_0-x_1)(x_0-x_2)} = \frac{(x-3)(x-4)}{(2-3)(2-4)} = \frac{(x-3)(x-4)}{2}$$

$$L_1 = \frac{(x-x_0)(x-x_2)}{(x_1-x_0)(x_1-x_2)} = \frac{(x-2)(x-4)}{(3-2)(3-4)} = \frac{(x-2)(x-4)}{-1}$$



$$L_2 = \frac{(x-x_0)(x-x_1)}{(x_2-x_0)(x_2-x_1)} = \frac{(x-2)(x-3)}{(4-2)(4-3)} = \frac{(x-2)(x-3)}{2}$$

$$P(x) = 0.6931 \cdot \frac{(x-3)(x-4)}{2} + 1.0986 \cdot \frac{(x-2)(x-4)}{-1} + 1.3863 \cdot \frac{(x-2)(x-3)}{2}$$

$$b) P(2.3) = 0.6931 \cdot \frac{(2.3-3)(2.3-4)}{2} + 1.0986 \cdot \frac{(2.3-2)(2.3-4)}{-1} +$$

$$1.3863 \cdot \frac{(2.3-2)(2.3-3)}{2} = 0.4124 + 0.5603 + (-0.1456) =$$

$$P(2.3) = \boxed{0.8271}$$

Passo 1:  $f^{(m+1)}(x) = f^{(3)}(x) = \ln(x)$

$|\ln(x)| \leq M$  para todo  $x \in (2,4)$

$x=4 \rightarrow |\ln(4)| = 1.3863$

$M \geq 1.3863$

Passo 2: Cálculo do erro

$$|E| \leq \sum_{k=0}^{m=2} \frac{|x-x_k|}{(m+1)!} M$$

$$|E| \leq \frac{|(2.3-2)(2.3-3)(2.3-4)|}{(2+1)!} \cdot 1.3863 =$$

$$\frac{|(0.3)(-0.7)(-1.7)|}{3!} \cdot 1.3863 = 0.357 \cdot \frac{1.3863}{6} =$$

$$0.357 \cdot 0.2311 = \boxed{0.0825}$$

O valor  $p(2.3) = 0.8271$  é uma aproximação para  $\ln(2.3)$  com erro  $\leq 0.0825$ .



$$P(3.3) = 0.6931 \cdot \frac{(3.3-3)(3.3-4)}{2} + 1.0986 \cdot \frac{(3.3-2)(3.3-4)}{-1} + 1.3863 \cdot \frac{(3.3-2)(3.3-3)}{2} = -0.0729 + 0.9997 + 0.2703 =$$

$$P(3.3) = \boxed{1.1972} //$$

passo 1:  $f^{(3)}(x) = \ln(x)$   $M \geq 1.3863$

passo 2:

$$|E| \leq \frac{1}{|(3.3-2)(3.3-3)(3.3-4)|} \cdot 0.2311 = \frac{1}{|(1.3)(0.3)(-0.7)|} \cdot 0.2311 = 0.273 \cdot 0.2311 =$$

$$|E| \leq \boxed{0.063}$$

O valor  $P(3.3) = 1.1972$  é uma aproximação para  $\ln(3.3)$  com erro  $\leq 0.063$ .